finished running example rpt

imp/example/Repeat.v
@@ -20,62 +20,6 @@ Set Implicit Arguments.
 
 Local Open Scope nat_scope.
 
-Module SUCC.
-
-  Definition succF : list val -> itree Es val :=
-    fun varg =>
-      n <- ((pargs [Tint] varg)?);;
-      Ret (Vint (n + 1)).
-
-  Definition succMS_ : ModSem._t :=
-    {|
-      ModSem.fnsems := [("succ", cfunU succF)];
-      ModSem.initial_st := tt↑;
-    |}.
-
-  Definition succMS : ModSem.t := Algebra.just succMS_.
-
-  Program Definition succM : Mod.t :=
-    {|
-      Mod.get_modsem := fun _ => succMS;
-      Mod.sk := Sk.unit;
-    |}.
-  Next Obligation. ss. Qed.
-  Next Obligation. ss. Qed.
-  Next Obligation. ss. Qed.
-
-  Lemma red_succF v: succF [Vint v] = Ret (Vint (v + 1)).
-  Proof. unfold succF. grind. Qed.
-
-End SUCC.
-
-Module PUT.
-
-  Definition putOnceF : list val -> itree Es val :=
-    fun varg =>
-      n <- ((pargs [Tint] varg)?);;
-      x <- trigger (Syscall "print" ((Vint n)↑) top1);;
-      Ret (Vint n).
-
-  Definition putMS_ : ModSem._t :=
-    {|
-      ModSem.fnsems := [("putOnce", cfunU putOnceF)];
-      ModSem.initial_st := tt↑;
-    |}.
-
-  Definition putMS : ModSem.t := Algebra.just putMS_.
-
-  Program Definition putM : Mod.t :=
-    {|
-      Mod.get_modsem := fun _ => putMS;
-      Mod.sk := Sk.unit;
-    |}.
-  Next Obligation. ss. Qed.
-  Next Obligation. ss. Qed.
-  Next Obligation. ss. Qed.
-
-End PUT.
-
 Module RPT0.
 
   Definition rptF : list val -> itree Es val :=
@@ -150,15 +94,22 @@ Module RPT1.
 
 End RPT1.
 
+
+Definition cast_val {X} (body: X -> itree Es Z): X -> itree Es val :=
+  fun '(varg) => vret <- body varg;; Ret (Vint vret).
+
+Definition cfunU_int {X} (body: X -> itree Es Z): Any.t -> itree Es Any.t :=
+  cfunU (cast_val body).
+
 Module ONE.
 
-  Definition oneMS_ (fn: string) (f: Any.t -> itree Es Any.t): ModSem._t :=
+  Definition oneMS_ (fn: string) (f: list val -> itree Es Z): ModSem._t :=
     {|
-      ModSem.fnsems := [(fn, f)];
+      ModSem.fnsems := [(fn, cfunU_int f)];
       ModSem.initial_st := tt↑;
     |}.
 
-  Definition oneMS (fn: string) (f: Any.t -> itree Es Any.t): ModSem.t :=
+  Definition oneMS (fn: string) (f: list val -> itree Es Z): ModSem.t :=
     Algebra.just (oneMS_ fn f).
 
   Program Definition oneM fn f : Mod.t :=
@@ -172,6 +123,28 @@ Module ONE.
 
 End ONE.
 
+Module SUCC.
+
+  Definition succF : list val -> itree Es Z :=
+    fun varg =>
+      n <- ((pargs [Tint] varg)?);;
+      Ret (n + 1)%Z.
+
+  Definition succM : Mod.t := ONE.oneM "succ" succF.
+
+End SUCC.
+
+Module PUT.
+
+  Definition putOnceF : list val -> itree Es Z :=
+    fun varg =>
+      n <- ((pargs [Tint] varg)?);;
+      x <- trigger (Syscall "print" ((Vint n)↑) top1);;
+      Ret (n).
+
+  Definition putM : Mod.t := ONE.oneM "putOnce" putOnceF.
+
+End PUT.
 
 
 Section PROOFSIM.
@@ -184,130 +157,58 @@ Section PROOFSIM.
   Lemma Z_to_nat_ge_one z: forall n, S n = Z.to_nat z -> (z >= 1)%Z.
   Proof. intros. unfold Z.to_nat in H. des_ifs. lia. Qed.
 
-  (* Definition cfunU_int {X} (body: X -> itree Es Z): Any.t -> itree Es Any.t := *)
-  (*   fun '(varg) => varg <- varg↓?;; vret <- body varg;; Ret (Vint vret)↑. *)
-
-  (* Definition simple_function (f: list val -> itree Es Z) := *)
-  (*   forall vs, f vs = focus_right (f vs). *)
-
-  (** Needs a way to handle paired states --- ex) focus_right *)
-  (* Lemma simple_rpt_sim *)
-  (*       (fn': string) (f': list val -> itree Es Z) *)
-  (*       (SIMPLE: simple_function (f')) *)
-  (*   : *)
-  (*   ModSemPair.sim (RPT1.rptMS fn' (cfunU_int f')) (RPT0.rptMS ⊕ (ONE.oneMS fn' (cfunU_int f'))). *)
-  (* Proof. *)
-  (*   Local Opaque String.eqb. *)
-  (*   ss. eapply mk. eapply (@top2_PreOrder unit). instantiate (1:= (fun _ '(src, tgt) => src = tgt)). *)
-  (*   { i. ss. des; clarify. exists (focus_left (T:=Any.t) ∘ cfunU RPT0.rptF). split. *)
-  (*     { left. f_equal. } *)
-  (*     ii. subst y. ginit. *)
-  (*     unfold_goal RPT1.rptF. unfold_goal RPT0.rptF. unfold_goal @cfunU. *)
-  (*     unfold_goal @cfunU_int. *)
-  (*     steps. *)
-  (*     destruct p0. unfold unptr, unint, unr in *. des_ifs_safe. ss; clarify. *)
-  (*     destruct (String.eqb_spec fn' s). *)
-  (*     2:{ steps. } *)
-  (*     clarify. *)
-  (*     steps. *)
-  (*     (* force_r. eexists; auto. steps. *) *)
-  (*     rename z0 into v. *)
-  (*     remember (Z.to_nat z) as n. *)
-  (*     revert x z v _UNWRAPU _ASSUME Heqn mrs_tgt. induction n; intros. *)
-  (*     { hexploit Z_to_nat_le_zero; eauto. intros. des_ifs. *)
-  (*       2:{ lia. } *)
-  (*       ss. steps. *)
-  (*       (* unfold lift_rel. exists w; auto. *) *)
-  (*     } *)
-  (*     { hexploit Z_to_nat_ge_one; eauto. intros ZRANGE. des_ifs. clear l. *)
-  (*       ss. *)
-  (*       unfold ccallU. steps. *)
-  (*       { right; left. instantiate (1:=focus_right (T:=Any.t) <*> cfunU_int f'). f_equal. } *)
-  (*       unfold_goal @cfunU_int. steps. *)
-  (*       guclo lbindC_spec. econs. *)
-  (*       { guclo lflagC_spec. econs. gfinal. right. rewrite <- SIMPLE. eapply self_sim_itree. *)
-  (*         all: auto. *)
-  (*       } *)
-  (*       (* rewrite ! SUCC.red_succF. steps. *) *)
-  (*       i. rr in SIM. des. clear WLE. clarify. destruct w1. steps. *)
-  (*       { left. instantiate (1:= focus_left (T:=Any.t) ∘ cfunU RPT0.rptF). auto. } *)
-  (*       unfold_goal @cfunU. steps. unfold_goal RPT0.rptF. steps. *)
-  (*       force_r. *)
-  (*       { exfalso. apply _ASSUME0. clear - _ASSUME ZRANGE. unfold_intrange_64. *)
-  (*         des_ifs. apply sumbool_to_bool_true in _ASSUME, H. *)
-  (*         apply andb_true_intro. split; apply sumbool_to_bool_is_true; lia. *)
-  (*       } *)
-  (*       steps. *)
-  (*       specialize (IHn ([Vptr (inr s) 0; Vint (z - 1); Vint (vret_tgt)]↑) (z - 1)%Z vret_tgt). *)
-  (*       exploit IHn; auto. *)
-  (*       { apply Any.upcast_downcast. } *)
-  (*       { lia. } *)
-  (*       clear IHn; intros IHn. des_ifs. *)
-  (*       { steps. *)
-  (*         match goal with *)
-  (*         | [IHn: gpaco8 _ _ _ _ _ _ _ _ _ _ _ (?t1) |- *)
-  (*              gpaco8 _ _ _ _ _ _ _ _ _ _ _ (?t2)] => *)
-  (*             replace t2 with t1 *)
-  (*         end. *)
-  (*         guclo lflagC_spec. econs. eapply IHn. *)
-  (*         all: auto. *)
-  (*         f_equal. ired_eq_l. auto. *)
-  (*       } *)
-  (*       { steps. irw in IHn. *)
-  (*         guclo guttC_spec. econs. *)
-  (*         { guclo lflagC_spec. econs. eapply IHn. all: auto. } *)
-  (*         - apply Reflexive_eqit_eq. *)
-  (*         - ired_eq_r. *)
-  (*           apply eqit_bind. apply Reflexive_eqit_eq. ii. *)
-  (*           apply eqit_bind. apply Reflexive_eqit_eq. ii. *)
-  (*           ired_eq_l. apply eqit_Tau_l. ired_eq_l. ired_eq_r. *)
-  (*           apply Reflexive_eqit_eq. *)
-  (*       } *)
-  (*     } *)
-  (*   } *)
-  (*   { ss. exists tt. auto. } *)
-  (* Qed. *)
-
-  Lemma succ_rpt_sim:
-    ModSemPair.sim (RPT1.rptMS "succ" (cfunU SUCC.succF)) (RPT0.rptMS ⊕ SUCC.succMS).
+  Lemma one_rpt_sim
+        (fn': string) (f': list val -> itree Es Z)
+    :
+    ModSemPair.sim (RPT1.rptMS fn' (cfunU_int f')) (RPT0.rptMS ⊕ (ONE.oneMS fn' f')).
   Proof.
     Local Opaque String.eqb.
-    ss. eapply mk. eapply Nat.le_preorder. instantiate (1:= fun _ _ => True).
+    ss. eapply mk. eapply (@top2_PreOrder unit). instantiate (1:= (fun _ '(src, tgt) => exists tgt_l, tgt = Any.pair tgt_l src)).
     { i. ss. des; clarify. exists (focus_left (T:=Any.t) ∘ cfunU RPT0.rptF). split.
       { left. f_equal. }
-      unfold RPT1.rptF. unfold RPT0.rptF at 2. unfold cfunU at 3 4.
-      unfold sim_fsem. ii. subst y.
-      ginit.
-      unfold cfunU at 5. steps.
+      ii. subst y. ginit.
+      unfold_goal RPT1.rptF. unfold_goal RPT0.rptF. unfold_goal @cfunU.
+      unfold_goal @cfunU_int. unfold_goal @cast_val.
+      steps.
       destruct p0. unfold unptr, unint, unr in *. des_ifs_safe. ss; clarify.
-      destruct (String.eqb_spec "succ" s).
+      destruct (String.eqb_spec fn' s).
       2:{ steps. }
       clarify.
       steps.
       (* force_r. eexists; auto. steps. *)
       rename z0 into v.
+      des; clarify.
       remember (Z.to_nat z) as n.
-      revert x z v _UNWRAPU _ASSUME Heqn. induction n; intros.
+      revert x z v _UNWRAPU _ASSUME Heqn mrs_src tgt_l. induction n; intros.
       { hexploit Z_to_nat_le_zero; eauto. intros. des_ifs.
         2:{ lia. }
-        ss. steps.  unfold lift_rel. exists w; auto.
+        ss. steps.
+        unfold lift_rel. exists w; splits; eauto.
       }
       { hexploit Z_to_nat_ge_one; eauto. intros ZRANGE. des_ifs. clear l.
         ss.
         unfold ccallU. steps.
-        { right; left. instantiate (1:=focus_right (T:=Any.t) ∘ cfunU SUCC.succF). f_equal. }
-        unfold cfunU at 5. steps.
-        rewrite ! SUCC.red_succF. steps.
+        { right; left. instantiate (1:=focus_right (T:=Any.t) <*> cfunU_int f'). f_equal. }
+        unfold_goal @cfunU_int. unfold_goal @cfunU. unfold_goal @cast_val. steps.
+        guclo lbindC_spec. econs.
+        { guclo lflagC_spec. econs. gfinal. right.
+          eapply sim_itree_fsubset. 2: eapply sim_itree_tgtr. ss. eapply self_sim_itree.
+          all: eauto.
+          i. ss. split; ii.
+          - des. clarify. eauto.
+          - des. clarify. eauto.
+        }
+        i. rr in SIM. des. clear WLE. clarify. destruct w1. steps.
         { left. instantiate (1:= focus_left (T:=Any.t) ∘ cfunU RPT0.rptF). auto. }
-        unfold cfunU at 5. steps. unfold RPT0.rptF at 3. steps.
+        unfold_goal @cfunU. steps. unfold_goal RPT0.rptF. steps.
         force_r.
         { exfalso. apply _ASSUME0. clear - _ASSUME ZRANGE. unfold_intrange_64.
           des_ifs. apply sumbool_to_bool_true in _ASSUME, H.
           apply andb_true_intro. split; apply sumbool_to_bool_is_true; lia.
         }
         steps.
-        specialize (IHn ([Vptr (inr "succ") 0; Vint (z - 1); Vint (v +1)]↑) (z - 1)%Z (v + 1)%Z).
-        hexploit IHn; auto.
+        specialize (IHn ([Vptr (inr s) 0; Vint (z - 1); Vint (vret_tgt)]↑) (z - 1)%Z vret_tgt).
+        exploit IHn; auto.
         { apply Any.upcast_downcast. }
         { lia. }
         clear IHn; intros IHn. des_ifs.
@@ -333,105 +234,26 @@ Section PROOFSIM.
         }
       }
     }
-    { ss. exists O. auto. }
+    { ss. exists tt. eauto. }
   Qed.
 
-  Lemma putOnce_rpt_sim:
-    ModSemPair.sim (RPT1.rptMS "putOnce" (cfunU PUT.putOnceF)) (RPT0.rptMS ⊕ PUT.putMS).
+  Theorem one_rpt_ref fn f:
+    (RPT0.rptM ⊕ (ONE.oneM fn f)) ⊑ (RPT1.rptM fn (cfunU_int f)).
   Proof.
-    Local Opaque String.eqb.
-    ss. eapply mk. eapply Nat.le_preorder. instantiate (1:= fun _ _ => True).
-    { i. ss. des; clarify. exists (focus_left (T:=Any.t) ∘ cfunU RPT0.rptF). split.
-      { left. f_equal. }
-      unfold RPT1.rptF. unfold RPT0.rptF at 2. unfold cfunU at 3 4.
-      unfold sim_fsem. ii. subst y.
-      ginit.
-      unfold cfunU at 5. steps.
-      destruct p0. unfold unptr, unint, unr in *. des_ifs_safe. ss; clarify.
-      destruct (String.eqb_spec "putOnce" s).
-      2:{ steps. }
-      clarify.
-      steps.
-      (* force_r. eexists; auto. steps. *)
-      rename z0 into v.
-      remember (Z.to_nat z) as n.
-      revert x z v _UNWRAPU _ASSUME Heqn. induction n; intros.
-      { hexploit Z_to_nat_le_zero; eauto. intros. des_ifs.
-        2:{ lia. }
-        ss. steps.  unfold lift_rel. exists w; auto.
-      }
-      { hexploit Z_to_nat_ge_one; eauto. intros ZRANGE. des_ifs. clear l.
-        ss.
-        unfold ccallU. steps.
-        { right; left. instantiate (1:=focus_right (T:=Any.t) ∘ cfunU PUT.putOnceF). f_equal. }
-        unfold cfunU at 5. steps.
-        unfold PUT.putOnceF at 3 5. steps.
-        { left. instantiate (1:= focus_left (T:=Any.t) ∘ cfunU RPT0.rptF). auto. }
-        unfold cfunU at 5. steps. unfold RPT0.rptF at 3. steps.
-        force_r.
-        { exfalso. apply _ASSUME0. clear - _ASSUME ZRANGE. unfold_intrange_64.
-          des_ifs. apply sumbool_to_bool_true in _ASSUME, H.
-          apply andb_true_intro. split; apply sumbool_to_bool_is_true; lia.
-        }
-        steps.
-        specialize (IHn ([Vptr (inr "putOnce") 0; Vint (z - 1); Vint (v)]↑) (z - 1)%Z (v)%Z).
-        hexploit IHn; auto.
-        { apply Any.upcast_downcast. }
-        { lia. }
-        clear IHn; intros IHn. des_ifs.
-        { steps.
-          match goal with
-          | [IHn: gpaco8 _ _ _ _ _ _ _ _ _ _ _ (?t1) |-
-               gpaco8 _ _ _ _ _ _ _ _ _ _ _ (?t2)] =>
-              replace t2 with t1
-          end.
-          guclo lflagC_spec. econs. eapply IHn.
-          all: auto.
-          f_equal. ired_eq_l. auto.
-        }
-        { steps. irw in IHn.
-          guclo guttC_spec. econs.
-          { guclo lflagC_spec. econs. eapply IHn. all: auto. }
-          - apply Reflexive_eqit_eq.
-          - ired_eq_r.
-            apply eqit_bind. apply Reflexive_eqit_eq. ii.
-            apply eqit_bind. apply Reflexive_eqit_eq. ii.
-            ired_eq_l. apply eqit_Tau_l. ired_eq_l. ired_eq_r.
-            apply Reflexive_eqit_eq.
-        }
-      }
-    }
-    { ss. exists O. auto. }
+    eapply LSimMod. ss. ss. i. eapply ModSemPair.adequacy. apply one_rpt_sim.
   Qed.
 
-  Theorem succ_rpt_ref: (RPT0.rptM ⊕ SUCC.succM) ⊑ (RPT1.rptM "succ" (cfunU SUCC.succF)).
-  Proof.
-    eapply LSimMod. ss. ss. i. eapply ModSemPair.adequacy. apply succ_rpt_sim.
-  Qed.
+  Theorem succ_rpt_ref:
+    (RPT0.rptM ⊕ SUCC.succM) ⊑ (RPT1.rptM "succ" (cfunU_int SUCC.succF)).
+  Proof. eapply one_rpt_ref. Qed.
 
-  Theorem putOnce_rpt_ref: (RPT0.rptM ⊕ PUT.putM) ⊑ (RPT1.rptM "putOnce" (cfunU PUT.putOnceF)).
-  Proof.
-    eapply LSimMod. ss. ss. i. eapply ModSemPair.adequacy. apply putOnce_rpt_sim.
-  Qed.
+  Theorem putOnce_rpt_ref:
+    (RPT0.rptM ⊕ PUT.putM) ⊑ (RPT1.rptM "putOnce" (cfunU_int PUT.putOnceF)).
+  Proof. eapply one_rpt_ref. Qed.
 
 End PROOFSIM.
 
 Section PROOF.
-
-  Lemma own_persistent (M: MRAS.t) (m: M)
-    :
-    (Own m) -∗ (□ Own ( | m | )).
-  Proof.
-    rr. econs. ii. rr. split.
-    { rr. auto. }
-    rr. rr in H. des. exists ( | ctx | ). rewrite <- bar_oplus. rewrite H. auto.
-  Qed.
-
-  Lemma ownm_persistent
-        (m: Mod.t)
-    :
-    (OwnM m) -∗ (□ OwnM ( | m | )).
-  Proof. eapply own_persistent. Qed.
 
   Lemma rpt0_core
     :
@@ -509,36 +331,37 @@ Section PROOF.
     iIntros "H". iPoseProof (rpt0_persistent with "H") as "H". auto.
   Qed.
 
-  Lemma succ_rpt_ref_iprop:
-    OwnM RPT0.rptM ∗ OwnM SUCC.succM ⊢ |==> OwnM (RPT1.rptM "succ" (cfunU SUCC.succF)).
+  Lemma rpt0_spec:
+    OwnM (RPT0.rptM) ⊢ □ (∀ fn f, OwnM (ONE.oneM fn f) ==∗ OwnM (RPT1.rptM fn (cfunU_int f))).
   Proof.
-    iIntros "[RPT0 SUCC]". iPoseProof (own_sep with "[SUCC RPT0]") as "OWN". iFrame.
-    iStopProof. apply IPM.adequacy. apply succ_rpt_ref.
+    iIntros "#RPT0". iModIntro. iIntros (fn f) "ONE".
+    iPoseProof (own_sep with "[ONE RPT0]") as "OWN". iSplitL "RPT0". auto. iApply "ONE".
+    iClear "RPT0".
+    iStopProof. apply IPM.adequacy. apply one_rpt_ref.
   Qed.
 
-  Lemma putOnce_rpt_ref_iprop:
-    OwnM RPT0.rptM ∗ OwnM PUT.putM ⊢ |==> OwnM (RPT1.rptM "putOnce" (cfunU PUT.putOnceF)).
-  Proof.
-    iIntros "[RPT0 PUT]". iPoseProof (own_sep with "[PUT RPT0]") as "OWN". iFrame.
-    iStopProof. apply IPM.adequacy. apply putOnce_rpt_ref.
-  Qed.
+  (** Coq complains that type is wrong. *)
+  (* Definition REF : mProp := *)
+  (*   ∀ (fn: string) (f: list val -> itree Es Z), *)
+  (*     OwnM (ONE.oneM fn f) ==∗ OwnM (RPT1.rptM fn (cfunU_int f)). *)
 
   Theorem rpts_ref_iprop:
     OwnM RPT0.rptM ∗ OwnM SUCC.succM ∗ OwnM PUT.putM
       ⊢
-      |==> ((OwnM (RPT1.rptM "succ" (cfunU SUCC.succF)))
-              ∗ (OwnM (RPT1.rptM "putOnce" (cfunU PUT.putOnceF)))).
+      |==> ((OwnM (RPT1.rptM "succ" (cfunU_int SUCC.succF)))
+              ∗ (OwnM (RPT1.rptM "putOnce" (cfunU_int PUT.putOnceF)))).
   Proof.
     iIntros "[#RPT0 [SUCC PUT]]".
-    iPoseProof (succ_rpt_ref_iprop with "[SUCC]") as "SUCCREF". iFrame. auto.
-    iPoseProof (putOnce_rpt_ref_iprop with "[PUT]") as "PUTREF". iFrame. auto.
+    iPoseProof (rpt0_spec with "RPT0") as "#RPT0_SPEC".
+    iPoseProof ("RPT0_SPEC" with "SUCC") as "SUCCREF".
+    iPoseProof ("RPT0_SPEC" with "PUT") as "PUTREF".
     iMod "SUCCREF". iMod "PUTREF". iModIntro. iFrame.
   Qed.
 
   Theorem rpts_ref:
     (RPT0.rptM ⊕ SUCC.succM ⊕ PUT.putM)
       ⊑
-      (RPT1.rptM "succ" (cfunU SUCC.succF)) ⊕ (RPT1.rptM "putOnce" (cfunU PUT.putOnceF)).
+      (RPT1.rptM "succ" (cfunU_int SUCC.succF)) ⊕ (RPT1.rptM "putOnce" (cfunU_int PUT.putOnceF)).
   Proof.
     pose proof rpts_ref_iprop. do 2 setoid_rewrite <- own_sep in H.
     eapply IPM.adequacy in H. rewrite oplus_assoc in H. eapply H.
